thys/Simpl/AlternativeSmallStep.thy
@@ -1158,25 +1158,6 @@ apply (rule not_infI)
 apply (rule_tac f=f in not_inf_Stuck')
 by auto
 
-lemma rtrancl_imp_rel_pow: "p \<in> R\<^sup>* \<Longrightarrow> \<exists>n. p \<in> R^^n"
-proof -
-  assume "p \<in> R\<^sup>*"
-  moreover obtain x y where p: "p = (x,y)" by (cases p)
-  ultimately have "(x,y) \<in> R\<^sup>*" by hypsubst
-  hence "\<exists>n. (x,y) \<in> R^^n"
-  proof (induct rule: rtrancl_induct)
-    fix a have "(a,a) \<in> R^^0" by simp
-    thus "\<exists>n. (a,a) \<in> R ^^ n" ..
-  next
-    fix a b c assume "\<exists>n. (a,b) \<in> R ^^ n"
-    then obtain n where "(a,b) \<in> R^^n" ..
-    moreover assume "(b,c) \<in> R"
-    ultimately have "(a,c) \<in> R^^(Suc n)" by auto
-    thus "\<exists>n. (a,c) \<in> R^^n" ..
-  qed
-  with p show ?thesis by hypsubst
-qed  
-
 lemma last_butlast_app: 
 assumes butlast: "butlast as = xs @ butlast bs"
 assumes not_Nil: "bs \<noteq> []" "as \<noteq> []"
